Add operations theory for two datatype with two binding position for one free position

operations/Least_Fixpoint2.thy
@@ -61,7 +61,6 @@ declare [[quick_and_dirty=false]]
 
 lemmas infinite_UNIV = cinfinite_imp_infinite[OF term_pre.UNIV_cinfinite]
 
-
 (********************** BINDER FIXPOINT CONSTRUCTION **************************************)
 
 typ "('a, 'b1, 'b2, 'brec1, 'brec2, 'rec) term_pre"
@@ -73,7 +72,7 @@ primrec permute_raw_term :: "('a::var_term_pre \<Rightarrow> 'a) \<Rightarrow> '
     map_term_pre id id id (permute_raw_term f) (permute_raw_term f) (permute_raw_term f) x
   ))"
 
-lemma permute_raw_simp:
+lemma permute_raw_simps:
   fixes f::"'a::var_term_pre \<Rightarrow> 'a"
   assumes "bij f" "|supp f| <o |UNIV::'a set|"
   shows "permute_raw_term f (raw_term_ctor x) = raw_term_ctor (map_term_pre f f f (permute_raw_term f) (permute_raw_term f) (permute_raw_term f) x)"
@@ -97,19 +96,59 @@ definition FVars_raw_term :: "'a::var_term_pre raw_term \<Rightarrow> 'a set" wh
 definition "suppGr f \<equiv> {(x, f x) | x. f x \<noteq> x}"
 
 coinductive alpha_term :: "'a::var_term_pre raw_term \<Rightarrow> 'a raw_term \<Rightarrow> bool" where
-  "\<lbrakk> bij g ; |supp g| <o |UNIV::'a set| ; suppGr f1 \<union> suppGr f2 \<subseteq> suppGr g ;
-    bij f1 ; |supp f1| <o |UNIV::'a set| ; id_on (\<Union>(FVars_raw_term ` set4_term_pre x) - (set2_term_pre x \<union> set3_term_pre x)) f1 ;
+  "\<lbrakk> bij g ; |supp g| <o |UNIV::'a set| ;
+    id_on (\<Union>(FVars_raw_term ` set4_term_pre x) - (set2_term_pre x \<union> set3_term_pre x)) g ;
     bij f2 ; |supp f2| <o |UNIV::'a set| ; id_on (\<Union>(FVars_raw_term ` set5_term_pre x) - set3_term_pre x) f2 ;
-    mr_rel_term_pre id g g (\<lambda>x. alpha_term (permute_raw_term f1 x)) (\<lambda>x. alpha_term (permute_raw_term f2 x)) alpha_term x y
+    eq_on (set3_term_pre x) f2 g ;
+    mr_rel_term_pre id g g (\<lambda>x. alpha_term (permute_raw_term g x)) (\<lambda>x. alpha_term (permute_raw_term f2 x)) alpha_term x y
   \<rbrakk> \<Longrightarrow> alpha_term (raw_term_ctor x) (raw_term_ctor y)"
 monos conj_context_mono term_pre.mr_rel_mono[OF supp_id_bound]
 
+type_synonym 'a raw_term_pre = "('a, 'a, 'a, 'a raw_term, 'a raw_term, 'a raw_term) term_pre"
+
+definition avoid_raw_term :: "'a::var_term_pre raw_term_pre \<Rightarrow> 'a set \<Rightarrow> 'a raw_term_pre" where
+  "avoid_raw_term x A \<equiv> SOME y. (set2_term_pre y \<union> set3_term_pre y) \<inter> A = {} \<and> alpha_term (raw_term_ctor x) (raw_term_ctor y)"
+
+typedef ('a::var_term_pre) "term" = "(UNIV::'a raw_term set) // { (x, y). alpha_term x y }"
+  apply (rule exI)
+  apply (rule quotientI)
+  apply (rule UNIV_I)
+  done
+
+abbreviation "TT_abs \<equiv> quot_type.abs alpha_term Abs_term"
+abbreviation "TT_rep \<equiv> quot_type.rep Rep_term"
+
+type_synonym 'a term_pre' = "('a, 'a, 'a, 'a term, 'a term, 'a term) term_pre"
+
+definition term_ctor :: "'a::var_term_pre term_pre' \<Rightarrow> 'a term" where
+  "term_ctor x \<equiv> TT_abs (raw_term_ctor (map_term_pre id id id TT_rep TT_rep TT_rep x))"
+
+definition permute_term :: "('a::var_term_pre \<Rightarrow> 'a) \<Rightarrow> 'a term \<Rightarrow> 'a term" where
+  "permute_term f x \<equiv> TT_abs (permute_raw_term f (TT_rep x))"
+
+definition FVars_term :: "'a::var_term_pre term \<Rightarrow> 'a set" where
+  "FVars_term x \<equiv> FVars_raw_term (TT_rep x)"
+
+definition avoid_term :: "'a::var_term_pre term_pre' \<Rightarrow> 'a set \<Rightarrow> 'a term_pre'" where
+  "avoid_term x A \<equiv> map_term_pre id id id TT_abs TT_abs TT_abs (
+    avoid_raw_term (map_term_pre id id id TT_rep TT_rep TT_rep x) A)"
+
+inductive subshape_term_term :: "'a::var_term_pre raw_term \<Rightarrow> 'a raw_term \<Rightarrow> bool" where
+  "\<lbrakk> bij f ; |supp f| <o |UNIV::'a set| ; alpha_term (permute_raw_term f y) z ;
+    z \<in> set4_term_pre x \<union> set5_term_pre x \<union> set6_term_pre x \<rbrakk> \<Longrightarrow> subshape_term_term y (raw_term_ctor x)"
+
+definition noclash_raw_term :: "'a::var_term_pre raw_term_pre \<Rightarrow> bool" where
+  "noclash_raw_term x \<equiv> (set2_term_pre x \<union> set3_term_pre x) \<inter> (set1_term_pre x \<union> \<Union>(FVars_raw_term ` set6_term_pre x)) = {}"
+
+definition noclash_term :: "'a::var_term_pre term_pre' \<Rightarrow> bool" where
+  "noclash_term x \<equiv> (set2_term_pre x \<union> set3_term_pre x) \<inter> (set1_term_pre x \<union> \<Union>(FVars_term ` set6_term_pre x)) = {}"
+
 (****************** PROOFS ******************)
 
-lemma permute_raw_id: "permute_raw_term id x = x"
+lemma permute_raw_ids: "permute_raw_term id x = x"
   apply (rule raw_term.induct[of _ x])
   apply (rule trans)
-   apply (rule permute_raw_simp)
+   apply (rule permute_raw_simps)
     apply (rule bij_id supp_id_bound)+
   apply (rule trans)
    apply (rule arg_cong[of _ _ raw_term_ctor])
@@ -120,19 +159,32 @@ lemma permute_raw_id: "permute_raw_term id x = x"
          apply (rule refl trans[OF _ id_apply[symmetric]] | assumption)+
   done
 
+lemmas permute_raw_id0s = permute_raw_ids[abs_def, unfolded id_def[symmetric], THEN meta_eq_to_obj_eq]
+
 lemma permute_raw_comps:
   fixes f::"'a::var_term_pre \<Rightarrow> 'a" and g::"'a \<Rightarrow> 'a"
   assumes f_prems: "bij f" "|supp f| <o |UNIV::'a set|"
     and g_prems: "bij g" "|supp g| <o |UNIV::'a set|"
   shows "permute_raw_term f (permute_raw_term g x) = permute_raw_term (f \<circ> g) x"
-  sorry
+  apply (rule raw_term.induct[of _ x])
+  apply (subst permute_raw_simps, (rule assms bij_comp supp_comp_bound infinite_UNIV)+)+
+  apply (subst term_pre.map_comp)
+      apply (rule assms)+
+  apply (rule arg_cong[OF term_pre.map_cong])
+                  apply (rule assms bij_comp supp_comp_bound infinite_UNIV refl)+
+    apply (rule trans[OF comp_apply], assumption)+
+  done
 
-lemma permute_raw_congs:
+lemma permute_raw_comp0s:
   fixes f::"'a::var_term_pre \<Rightarrow> 'a" and g::"'a \<Rightarrow> 'a"
   assumes f_prems: "bij f" "|supp f| <o |UNIV::'a set|"
     and g_prems: "bij g" "|supp g| <o |UNIV::'a set|"
-  shows "(\<And>a. a \<in> FVars_raw_term x \<Longrightarrow> f a = g a) \<Longrightarrow> permute_raw_term f x = permute_raw_term g x"
-  sorry
+  shows "permute_raw_term f \<circ> permute_raw_term g = permute_raw_term (f \<circ> g)"
+  apply (rule ext)
+  apply (rule trans[OF comp_apply])
+  apply (rule permute_raw_comps)
+     apply (rule assms)+
+  done
 
 lemma FVars_raw_intros:
   "a \<in> set1_term_pre x \<Longrightarrow> a \<in> FVars_raw_term (raw_term_ctor x)"
@@ -143,7 +195,132 @@ lemma FVars_raw_intros:
      apply (erule free_raw_term.intros | assumption)+
   done
 
-lemma alpha_refl:
+lemma FVars_raw_ctors:
+  "FVars_raw_term (raw_term_ctor x) = set1_term_pre x \<union> (\<Union>(FVars_raw_term ` set4_term_pre x) - (set2_term_pre x \<union> set3_term_pre x))
+   \<union> (\<Union>(FVars_raw_term ` set5_term_pre x) - set3_term_pre x) \<union> \<Union>(FVars_raw_term ` set6_term_pre x)"
+  apply (rule subset_antisym)
+   apply (unfold FVars_raw_term_def)[1]
+   apply (rule subsetI)
+   apply (unfold mem_Collect_eq)
+   apply (erule free_raw_term.cases)
+      (* REPEAT_DETERM *)
+      apply (drule iffD1[OF raw_term.inject])
+      apply hypsubst_thin
+      apply (tactic \<open>resolve_tac @{context} [BNF_Util.mk_UnIN 4 1] 1\<close>)
+      apply assumption
+    (* repeated *)
+     apply (drule iffD1[OF raw_term.inject])
+     apply hypsubst_thin
+     apply (tactic \<open>resolve_tac @{context} [BNF_Util.mk_UnIN 4 2] 1\<close>)
+     apply (rule DiffI)
+      apply (rule UN_I)
+       apply (unfold mem_Collect_eq)
+       apply assumption+
+    (* repeated *)
+     apply (drule iffD1[OF raw_term.inject])
+     apply hypsubst_thin
+     apply (tactic \<open>resolve_tac @{context} [BNF_Util.mk_UnIN 4 3] 1\<close>)
+     apply (rule DiffI)
+      apply (rule UN_I)
+       apply (unfold mem_Collect_eq)
+       apply assumption+
+    (* repeated *)
+     apply (drule iffD1[OF raw_term.inject])
+     apply hypsubst_thin
+     apply (tactic \<open>resolve_tac @{context} [BNF_Util.mk_UnIN 4 4] 1\<close>)
+      apply (rule UN_I)
+       apply (unfold mem_Collect_eq)
+       apply assumption+
+    (* END REPEAT_DETERM *)
+  apply (rule subsetI)
+  apply (erule UnE)+
+     apply (((erule DiffE UN_E)+)?, erule FVars_raw_intros, (assumption+)?)+
+  done
+
+lemma FVars_raw_permute_leq:
+  fixes f::"'a::var_term_pre \<Rightarrow> 'a"
+  assumes f_prems: "bij f" "|supp f| <o |UNIV::'a set|"
+  shows "free_raw_term a x \<Longrightarrow> f a \<in> FVars_raw_term (permute_raw_term f x)"
+  apply (erule free_raw_term.induct[of _ x])
+  (* REPEAT_DETERM *)
+     apply (unfold permute_raw_simps[OF assms] FVars_raw_ctors)[1]
+     apply (subst term_pre.set_map, (rule assms supp_id_bound bij_id)+)+
+     apply (unfold image_comp[unfolded comp_def])
+             apply (tactic \<open>resolve_tac @{context} [BNF_Util.mk_UnIN 4 1] 1\<close>)
+     apply (rule DiffI)?
+     apply (rule imageI | (rule UN_I, assumption))
+     apply assumption
+    apply (rule iffD2[OF arg_cong[OF inj_image_mem_iff[OF bij_is_inj]]], rule assms, assumption)?
+  (* repeated *)
+     apply (unfold permute_raw_simps[OF assms] FVars_raw_ctors)[1]
+     apply (subst term_pre.set_map, (rule assms supp_id_bound bij_id)+)+
+     apply (unfold image_comp[unfolded comp_def])
+             apply (tactic \<open>resolve_tac @{context} [BNF_Util.mk_UnIN 4 2] 1\<close>)
+    apply (rule DiffI)?
+     apply (rule imageI | (rule UN_I, assumption))
+     apply assumption
+    apply (unfold image_Un[symmetric])[1]
+    apply (rule iffD2[OF arg_cong[OF inj_image_mem_iff[OF bij_is_inj]]], rule assms, assumption)?
+  (* repeated *)
+     apply (unfold permute_raw_simps[OF assms] FVars_raw_ctors)[1]
+     apply (subst term_pre.set_map, (rule assms supp_id_bound bij_id)+)+
+     apply (unfold image_comp[unfolded comp_def])
+             apply (tactic \<open>resolve_tac @{context} [BNF_Util.mk_UnIN 4 3] 1\<close>)
+    apply (rule DiffI)?
+     apply (rule imageI | (rule UN_I, assumption))
+     apply assumption
+    apply ((unfold image_Un[symmetric])[1])?
+    apply (rule iffD2[OF arg_cong[OF inj_image_mem_iff[OF bij_is_inj]]], rule assms, assumption)?
+  (* repeated *)
+     apply (unfold permute_raw_simps[OF assms] FVars_raw_ctors)[1]
+     apply (subst term_pre.set_map, (rule assms supp_id_bound bij_id)+)+
+     apply (unfold image_comp[unfolded comp_def])
+             apply (tactic \<open>resolve_tac @{context} [BNF_Util.mk_UnIN 4 4] 1\<close>)
+    apply (rule DiffI)?
+     apply (rule imageI | (rule UN_I, assumption))
+     apply assumption
+    apply ((unfold image_Un[symmetric])[1])?
+    apply (rule iffD2[OF arg_cong[OF inj_image_mem_iff[OF bij_is_inj]]], rule assms, assumption)?
+  (* END REPEAT_DETERM *)
+  done
+
+lemma FVars_raw_permutes:
+  fixes f::"'a::var_term_pre \<Rightarrow> 'a"
+  assumes f_prems: "bij f" "|supp f| <o |UNIV::'a set|"
+  shows "FVars_raw_term (permute_raw_term f x) = f ` FVars_raw_term x"
+  apply (rule subset_antisym)
+   apply (rule subsetI)
+   apply (subst (asm) FVars_raw_term_def)
+   apply (drule iffD1[OF mem_Collect_eq])
+   apply (drule FVars_raw_permute_leq[rotated -1])
+     prefer 3 (* 2 * nvars + 1 *)
+     apply (subst (asm) permute_raw_comps)
+         prefer 5 (* 4 * nvars + 1 *)
+         apply (subst (asm) inv_o_simp1, rule assms)+
+         apply (unfold permute_raw_ids)
+         apply (erule iffD2[OF image_in_bij_eq, rotated])
+         apply (rule assms bij_imp_bij_inv supp_inv_bound)+
+  apply (rule subsetI)
+  apply (erule imageE)
+  apply hypsubst
+  apply (subst (asm) FVars_raw_term_def)
+  apply (drule iffD1[OF mem_Collect_eq])
+  apply (erule FVars_raw_permute_leq[rotated -1])
+   apply (rule assms)+
+  done
+
+lemmas Un_bound = infinite_regular_card_order_Un[OF term_pre.bd_infinite_regular_card_order]
+lemmas UN_bound = regularCard_UNION_bound[OF term_pre.bd_Cinfinite term_pre.bd_regularCard]
+
+lemma FVars_raw_bds: "|FVars_raw_term x| <o natLeq"
+  apply (rule raw_term.induct[of _ x])
+  apply (unfold FVars_raw_ctors)
+  apply (rule Un_bound term_pre.set_bd ordLeq_ordLess_trans[OF card_of_diff] UN_bound | assumption)+
+  done
+
+lemmas FVars_raw_bd_UNIVs = FVars_raw_bds[THEN ordLess_ordLeq_trans, OF var_term_pre_class.large]
+
+lemma alpha_refls:
   fixes x::"'a::var_term_pre raw_term"
   shows "alpha_term x x"
 proof -
@@ -156,13 +333,8 @@ proof -
       apply (rule raw_term.exhaust[of x])
       apply hypsubst_thin
       apply (rule exI)+
-      apply (rule conjI, rule refl supp_id_bound bij_id id_on_id)+
-      apply (rule conjI)
-       apply (rule subsetI)
-       apply (erule UnE)+
-        apply assumption+
-      apply (rule conjI, rule refl supp_id_bound bij_id id_on_id)+
-      apply (unfold term_pre.mr_rel_id[symmetric] permute_raw_id)
+      apply (rule conjI, rule refl supp_id_bound bij_id id_on_id eq_on_refl)+
+      apply (unfold term_pre.mr_rel_id[symmetric] permute_raw_ids)
       apply (rule term_pre.rel_refl_strong)
         apply (rule disjI1 refl)+
       done
@@ -171,52 +343,11 @@ proof -
   show ?thesis by (rule x[THEN spec, THEN spec, THEN mp[OF _ refl]])
 qed
 
-lemma suppGr_inv: "bij f \<Longrightarrow> bij g \<Longrightarrow> suppGr f \<subseteq> suppGr g \<Longrightarrow> suppGr (inv f) \<subseteq> suppGr (inv g)"
-  unfolding suppGr_def using bij_imp_inv[of f] bij_imp_inv[of g] 
-  apply auto
-  subgoal 
-  proof -
-    fix x :: 'a
-    assume a1: "bij f"
-    assume a2: "bij g"
-    assume a3: "{(x, f x) |x. f x \<noteq> x} \<subseteq> {(x, g x) |x. g x \<noteq> x}"
-    assume "\<And>a. (inv f a = a) = (f a = a)"
-    assume a4: "f x \<noteq> x"
-    have "\<forall>a f. (\<exists>aa. (\<forall>ab. (aa::'a) = ab \<or> f ab \<noteq> (a::'a)) \<and> f aa = a) \<or> \<not> bij f"
-      by (metis (no_types) bij_pointE)
-    then obtain aa :: "'a \<Rightarrow> ('a \<Rightarrow> 'a) \<Rightarrow> 'a" and aaa :: "'a \<Rightarrow> ('a \<Rightarrow> 'a) \<Rightarrow> 'a" where
-      f5: "\<forall>a f. (\<forall>ab. aa a f = ab \<or> f ab \<noteq> a) \<and> f (aa a f) = a \<or> \<not> bij f"
-      by moura
-    then have "\<exists>a. (aa x f, x) = (a, g a) \<and> g a \<noteq> a"
-      using a4 a3 a1 by (smt (z3) mem_Collect_eq subset_iff)
-    then show "inv f x = inv g x"
-      using f5 a2 a1 by (metis (no_types) Pair_inject inv_simp1)
-  qed
-  by blast
-
-lemma suppGr_comp:
-  assumes "bij h1" "bij g" "bij f" "suppGr f \<subseteq> suppGr g"
-  shows "suppGr (h1 \<circ> f) \<subseteq> suppGr (h1 \<circ> g)"
-proof -
-  { fix x
-    assume a: "h1 (f x) \<noteq> x"
-    have "h1 (g x) = h1 (f x)"
-    proof (cases "f x = x")
-      case False
-      then show ?thesis using a assms(4) unfolding suppGr_def by auto
-    next
-      case True
-      then show ?thesis sorry
-    qed
-  }
-  then show ?thesis unfolding suppGr_def by auto
-qed
-
-lemma alpha_bij:
-  fixes f::"'a::var_term_pre \<Rightarrow> 'a" and g::"'a \<Rightarrow> 'a" and f2'::"'a \<Rightarrow> 'a"
-  assumes f_prems: "bij h1" "|supp h1| <o |UNIV::'a set|"
-    and g_prems: "bij h2" "|supp h2| <o |UNIV::'a set|"
-  shows "eq_on (FVars_raw_term x) h1 h2 \<Longrightarrow> alpha_term x y \<Longrightarrow> alpha_term (permute_raw_term h1 x) (permute_raw_term h2 y)"
+lemma alpha_bijs:
+  fixes f::"'a::var_term_pre \<Rightarrow> 'a" and g::"'a \<Rightarrow> 'a"
+  assumes f_prems: "bij f" "|supp f| <o |UNIV::'a set|"
+    and g_prems: "bij g" "|supp g| <o |UNIV::'a set|"
+  shows "eq_on (FVars_raw_term x) f g \<Longrightarrow> alpha_term x y \<Longrightarrow> alpha_term (permute_raw_term f x) (permute_raw_term g y)"
 proof -
   have x: "\<forall>(x::'a raw_term) y. (\<exists>x' y' f g. bij f \<and> |supp f| <o |UNIV::'a set| \<and> bij g \<and> |supp g| <o |UNIV::'a set|
     \<and> x = permute_raw_term f x' \<and> y = permute_raw_term g y' \<and> eq_on (FVars_raw_term x') f g \<and> alpha_term x' y')
@@ -227,90 +358,1443 @@ proof -
     apply (erule alpha_term.cases)
     apply hypsubst
     apply (unfold triv_forall_equality)
-    subgoal for h1 h2 g f1 f2 x y
-
-      thm ex_avoiding_bij[of f1 "\<Union> (FVars_raw_term ` set5_term_pre x) - set3_term_pre x" "set3_term_pre x"]
-
-      apply (subgoal_tac "bij f2'")
-       apply (subgoal_tac "|supp (f2'::'a \<Rightarrow> 'a)| <o |UNIV::'a set|")
-      apply (subgoal_tac "eq_on (\<Union> (FVars_raw_term ` set5_term_pre x)) f2' f2")
-      apply (rule exI[of _ "h2 \<circ> g \<circ> inv h1"])
-      apply (rule exI[of _ "h2 \<circ> f1' \<circ> inv h1"])
-      apply (rule exI[of _ "h2 \<circ> f2' \<circ> inv h1"])
+    subgoal for f g \<sigma> x f2 y
+      apply (rule exI[of _ "g \<circ> \<sigma> \<circ> inv f"])
+      apply (rule exI)
+      apply (rule exI[of _ "g \<circ> f2 \<circ> inv f"])
       apply (rule exI)+
-      apply (rule conjI, rule permute_raw_simp, (rule supp_id_bound bij_id | assumption)+)+
+      apply (rule conjI, rule permute_raw_simps, (rule supp_id_bound bij_id | assumption)+)+
       apply (rule conjI, (rule bij_comp supp_comp_bound bij_imp_bij_inv supp_inv_bound infinite_UNIV | assumption)+)+
 
-      apply (rule conjI[rotated])+
-             apply (rule iffD2[OF term_pre.mr_rel_map(1)])
-                       apply (assumption | rule supp_id_bound bij_id bij_comp supp_comp_bound infinite_UNIV bij_imp_bij_inv supp_inv_bound)+
-             apply (unfold id_o o_id)
-             apply (rule iffD2[OF term_pre.mr_rel_map(3)])
-                        apply (assumption | rule supp_id_bound bij_id bij_comp supp_comp_bound infinite_UNIV bij_imp_bij_inv supp_inv_bound)+
-             apply (unfold comp_assoc inv_id id_o o_id Grp_UNIV_id conversep_eq OO_eq relcompp_conversep_Grp Grp_OO)
-             apply (subst inv_o_simp1, assumption)+
-             apply (unfold id_o o_id comp_assoc[symmetric])
-             apply (subst inv_o_simp1, assumption)+
-             apply (unfold id_o o_id)
-             apply (erule term_pre.mr_rel_mono_strong0[rotated -7])
+      apply (subst term_pre.set_map, assumption+)+
+      apply (unfold image_Un[symmetric] image_comp[unfolded comp_def])
+      apply (subst FVars_raw_permutes, assumption+)+
+      apply (unfold image_UN[symmetric])
+      apply (subst image_set_diff[OF bij_is_inj, symmetric], assumption+)+
+
+      apply (rule conjI)
+       apply (rule id_onI)
+       apply (erule imageE)
+       apply hypsubst
+       apply (rule trans[OF comp_apply])
+       apply (rule trans[OF arg_cong[OF inv_simp1]])
+        apply assumption
+       apply (rule trans[OF comp_apply])
+       apply (rule trans[OF arg_cong[of _ _ g]])
+        apply (erule id_onD)
+        apply assumption
+       apply (rule sym)
+       apply (erule eq_onD)
+       apply (erule DiffE)
+       apply (erule UN_E)
+       apply (erule FVars_raw_intros)
+        apply assumption+
+
+      apply (rule conjI, (rule bij_comp supp_comp_bound bij_imp_bij_inv supp_inv_bound infinite_UNIV | assumption)+)+
+
+      apply (rule conjI)
+       apply (rule id_onI)
+       apply (erule imageE)
+       apply hypsubst
+       apply (rule trans[OF comp_apply])
+       apply (rule trans[OF arg_cong[OF inv_simp1]])
+        apply assumption
+       apply (rule trans[OF comp_apply])
+       apply (rule trans[OF arg_cong[of _ _ g]])
+        apply (erule id_onD)
+        apply assumption
+       apply (rule sym)
+       apply (erule eq_onD)
+       apply (erule DiffE)
+       apply (erule UN_E)
+       apply (erule FVars_raw_intros)
+        apply assumption+
+
+      apply (rule conjI)
+       apply (rule eq_on_comp)
+        apply (unfold image_comp inv_o_simp1 image_id)[1]
+        apply (rule eq_on_comp)
+         apply (rule eq_on_refl)
+        apply assumption
+      apply (rule eq_on_refl)
+
+      apply (rule iffD2[OF term_pre.mr_rel_map(1)])
+                apply (assumption | rule supp_id_bound bij_id bij_comp supp_comp_bound infinite_UNIV bij_imp_bij_inv supp_inv_bound)+
+      apply (unfold id_o o_id)
+      apply (rule iffD2[OF term_pre.mr_rel_map(3)])
+                 apply (assumption | rule supp_id_bound bij_id bij_comp supp_comp_bound infinite_UNIV bij_imp_bij_inv supp_inv_bound)+
+      apply (unfold comp_assoc inv_id id_o o_id Grp_UNIV_id conversep_eq OO_eq relcompp_conversep_Grp Grp_OO)
+      apply (subst inv_o_simp1, assumption)+
+      apply (unfold id_o o_id comp_assoc[symmetric])
+      apply (subst inv_o_simp1, assumption)+
+      apply (unfold id_o o_id)
+      apply (erule term_pre.mr_rel_mono_strong0[rotated -7])
         (* REPEAT_DETERM *)
-                          apply (rule ballI)
-                          apply (rule trans)
-                          apply (rule id_apply)
-                          apply (rule sym)
-                          apply (rule trans[OF comp_apply])
-                          apply (rule inv_f_eq[OF bij_is_inj])
-                          apply assumption
-                          apply (rule sym)
-                          apply (erule eq_onD)
-                          apply (erule FVars_raw_intros)
+                     apply (rule ballI)
+                     apply (rule trans)
+                      apply (rule id_apply)
+                     apply (rule sym)
+                     apply (rule trans[OF comp_apply])
+                     apply (rule inv_f_eq[OF bij_is_inj])
+                      apply assumption
+                     apply (rule sym)
+                     apply (erule eq_onD)
+                     apply (erule FVars_raw_intros)
         (* END REPEAT_DETERM *)
-                          apply (rule ballI, rule refl)+
-      prefer 2
-      (* REPEAT_DETERM *)
-                         apply (rule ballI)
-                         apply (rule ballI)
-                         apply (rule impI)
-      apply (rule disjI1)
-                         apply (rule exI)
-                         apply (rule exI)
-                         apply (rule exI[of _ h2])
-                         apply (rule exI[of _ h2])
-                         apply (rule conjI, assumption)+
-                         apply (rule conjI[rotated])+
-                          apply assumption
-                          apply (rule eq_on_refl)
-                          apply (rule refl)
-      apply (rule trans)
-                          apply (rule permute_raw_comps)
-                        apply (assumption | rule supp_id_bound bij_id bij_comp supp_comp_bound infinite_UNIV bij_imp_bij_inv supp_inv_bound)+
-                         apply (unfold comp_assoc)
-                         apply (subst inv_o_simp1, assumption)
-                         apply (unfold o_id)
-                         apply (rule trans)
-                          apply (rule permute_raw_comps[symmetric])
+                    apply (rule ballI, rule refl)+
+        (* REPEAT_DETERM *)
+                  apply (rule ballI)
+                  apply (rule ballI)
+                  apply (rule impI)
+                  apply (rule disjI1)
+                  apply (rule exI)+
+                  apply (rule conjI[rotated])+
+                         apply assumption
+                        apply (rule eq_on_refl)
+                       apply (rule refl)
+                      apply (rule trans)
+                       apply (rule permute_raw_comps)
                           apply (assumption | rule supp_id_bound bij_id bij_comp supp_comp_bound infinite_UNIV bij_imp_bij_inv supp_inv_bound)+
-                         apply (rule arg_cong[of _ _ "permute_raw_term h2"])
-                         apply (rule permute_raw_congs)
-                          apply assumption+
-                          apply (erule eq_onD)
-                          apply (rule UN_I)
-                          apply assumption+
+                      apply (unfold comp_assoc)
+                      apply (subst inv_o_simp1, assumption)
+                      apply (unfold o_id)
+                      apply (rule trans)
+                       apply (rule permute_raw_comps[symmetric])
+                          apply (assumption | rule supp_id_bound bij_id bij_comp supp_comp_bound infinite_UNIV bij_imp_bij_inv supp_inv_bound)+
+                      apply (rule refl)
+                     apply assumption+
+        (* repeated *)
+                  apply (rule ballI)
+                  apply (rule ballI)
+                  apply (rule impI)
+                  apply (rule disjI1)
+                  apply (rule exI)+
+                  apply (rule conjI[rotated])+
+                         apply assumption
+                        apply (rule eq_on_refl)
+                       apply (rule refl)
+                      apply (rule trans)
+                       apply (rule permute_raw_comps)
+                          apply (assumption | rule supp_id_bound bij_id bij_comp supp_comp_bound infinite_UNIV bij_imp_bij_inv supp_inv_bound)+
+                      apply (unfold comp_assoc)
+                      apply (subst inv_o_simp1, assumption)
+                      apply (unfold o_id)
+                      apply (rule trans)
+                       apply (rule permute_raw_comps[symmetric])
+                          apply (assumption | rule supp_id_bound bij_id bij_comp supp_comp_bound infinite_UNIV bij_imp_bij_inv supp_inv_bound)+
+                      apply (rule refl)
+                     apply assumption+
+        (* repeated, rec free case *)
+                  apply (rule ballI)
+                  apply (rule ballI)
+                  apply (rule impI)
+                  apply (rule disjI1)
+                apply (rule exI)+
+                  apply (rule conjI[rotated])+
+                       apply assumption
+                      apply (erule eq_on_mono[rotated -1])
+                      apply (rule subsetI)
+                      apply (erule FVars_raw_intros)
+                      apply assumption
+                     apply (rule refl)+
+                   apply assumption+
+            (* END REPEAT_DETERM *)
+               apply (rule supp_id_bound bij_id supp_comp_bound bij_comp infinite_UNIV supp_inv_bound bij_imp_bij_inv | assumption)+
+      done
+    done
 
-
-
+  show "eq_on (FVars_raw_term x) f g \<Longrightarrow> alpha_term x y \<Longrightarrow> alpha_term (permute_raw_term f x) (permute_raw_term g y)"
+    apply (rule x[THEN spec, THEN spec, THEN mp])
+    apply (rule exI)+
+    apply (rule conjI[rotated])+
+           apply assumption+
+         apply (rule refl)+
+       apply (rule assms)+
+    done
 qed
 
+lemma alpha_bij_eqs:
+  fixes f::"'a::var_term_pre \<Rightarrow> 'a" and g::"'a \<Rightarrow> 'a"
+  assumes f_prems: "bij f" "|supp f| <o |UNIV::'a set|"
+  shows "alpha_term (permute_raw_term f x) (permute_raw_term f y) = alpha_term x y"
+  apply (rule iffI)
+   apply (drule alpha_bijs[rotated -1])
+        prefer 6 (* 5 * nvars + 1 *)
+    (* REPEAT_DETERM *)
+        apply (subst (asm) permute_raw_comps)
+            prefer 5 (* 4 * nvars + 1 *)
+            apply (subst (asm) inv_o_simp1, rule assms)
+    (* repeated *)
+            apply (subst (asm) permute_raw_comps)
+                prefer 5 (* 4 * nvars + 1 *)
+                apply (subst (asm) inv_o_simp1, rule assms)
+    (* END REPEAT_DETERM *)
+                apply (unfold permute_raw_ids)
+                apply assumption
+               apply (rule bij_imp_bij_inv supp_inv_bound assms)+
+   apply (rule eq_on_refl)
+  apply (erule alpha_bijs[rotated -1])
+      apply (rule assms eq_on_refl)+
+  done
 
+lemma alpha_bij_eq_invs:
+  fixes f::"'a::var_term_pre \<Rightarrow> 'a" and g::"'a \<Rightarrow> 'a"
+  assumes f_prems: "bij f" "|supp f| <o |UNIV::'a set|"
+  shows "alpha_term (permute_raw_term f x) y = alpha_term x (permute_raw_term (inv f) y)"
+  apply (rule trans)
+   apply (rule alpha_bij_eqs[symmetric])
+    prefer 3 (* 2 * nvars + 1 *)
+    apply (subst permute_raw_comps)
+        prefer 5 (* 4 * nvars + 1 *)
+        apply (subst inv_o_simp1, rule assms)+
+        apply (unfold permute_raw_ids)
+        apply (rule refl)
+       apply (rule assms bij_imp_bij_inv supp_inv_bound)+
+  done
 
+lemma alpha_FVars: "alpha_term x y \<Longrightarrow> FVars_raw_term x = FVars_raw_term y"
+proof -
+  have x: "\<forall>y. alpha_term x y \<longrightarrow> FVars_raw_term x = FVars_raw_term y"
+    apply (rule raw_term.induct[of _ x])
+    subgoal premises IHs for x
+      apply (rule allI)
+      apply (rule impI)
+      apply (erule alpha_term.cases)
+      apply (drule iffD1[OF raw_term.inject])
+      apply hypsubst
+      apply (unfold FVars_raw_ctors)
+      apply (rule arg_cong2[of _ _ _ _ "(\<union>)"])+
+         apply (rule sym)
+         apply (erule term_pre.mr_rel_set[OF supp_id_bound, unfolded image_id, rotated -1])
+            apply (rule supp_id_bound bij_id | assumption)+
+        (* REPEAT_DETERM *)
+        apply (rule sym)
+        apply (rule trans)
+         apply (rule arg_cong2[of _ _ _ _ minus, rotated])
+           apply (rule arg_cong2[of _ _ _ _ "(\<union>)"])+
+            apply (erule term_pre.mr_rel_set[rotated -1], (rule supp_id_bound bij_id | assumption)+)+
+         prefer 2
+          apply (unfold image_Un[symmetric])[1]
+         apply (rule trans)
+          apply (rule image_set_diff[OF bij_is_inj, symmetric])
+          apply assumption
+         apply (erule id_on_image)
+        apply (unfold image_UN)[1]
+        apply (rule sym)
+        apply (rule rel_set_UN_D)
+        apply (erule term_pre.mr_set_transfer[THEN rel_funD, rotated -1, OF term_pre.mr_rel_mono_strong[rotated -4]])
+        (* REPEAT_DETERM *)
+                    apply (rule ballI)
+                    apply (rule ballI)
+                    apply (rule impI)
+                    apply (drule IHs)
+                    apply (drule alpha_bij_eq_invs[THEN iffD1, rotated -1])
+                      apply assumption+
+                    apply (erule allE)
+                    apply (erule impE)
+                     apply assumption
+                    apply (rule trans)
+                     apply (erule arg_cong[of _ _ "(`) _"])
+                    apply (subst FVars_raw_permutes)
+                      apply (rule bij_imp_bij_inv supp_inv_bound | assumption)+
+                    apply (unfold image_comp inv_o_simp2 image_id)
+                    apply (rule refl)
+        (* ORELSE *)
+                   apply (rule ballI, rule ballI, rule imp_refl)+
+        (* END REPEAT_DETERM *)
+                 apply (rule supp_id_bound bij_id | assumption)+
+        (* repeated *)
+       apply (rule sym)
+       apply (rule trans)
+        apply (rule arg_cong2[of _ _ _ _ minus, rotated])
+         apply (rule trans)
+          apply (erule term_pre.mr_rel_set[rotated -1], (rule supp_id_bound bij_id | assumption)+)+
+         apply (rule sym)
+         apply (erule eq_on_image)
+        prefer 2
+        apply (rule trans)
+         apply (rule image_set_diff[OF bij_is_inj, symmetric])
+         apply assumption
+        apply (erule id_on_image)
+       apply (unfold image_UN)[1]
+       apply (rule sym)
+       apply (rule rel_set_UN_D)
+       apply (erule term_pre.mr_set_transfer[THEN rel_funD, rotated -1, OF term_pre.mr_rel_mono_strong[rotated -4]])
+        (* REPEAT_DETERM *)
+                   apply (rule ballI, rule ballI, rule imp_refl)+
+        (* ORELSE *)
+                  apply (rule ballI)
+                  apply (rule ballI)
+                  apply (rule impI)
+                  apply (drule IHs)
+                  apply (drule alpha_bij_eq_invs[THEN iffD1, rotated -1])
+                    apply assumption+
+                  apply (erule allE)
+                  apply (erule impE)
+                   apply assumption
+                  apply (rule trans)
+                   apply (erule arg_cong[of _ _ "(`) _"])
+                  apply (subst FVars_raw_permutes)
+                    apply (rule bij_imp_bij_inv supp_inv_bound | assumption)+
+                  apply (unfold image_comp inv_o_simp2 image_id)
+                  apply (rule refl)
+        (* ORELSE *)
+                 apply (rule ballI, rule ballI, rule imp_refl)+
+        (* END REPEAT_DETERM *)
+                apply (rule supp_id_bound bij_id | assumption)+
+        (* repeated, rec free case *)
+      apply (rule rel_set_UN_D)
+      apply (erule term_pre.mr_set_transfer[THEN rel_funD, rotated -1, OF term_pre.mr_rel_mono_strong[rotated -4]])
+                  apply (rule ballI, rule ballI, rule imp_refl)+
+        (* ORELSE *)
+                apply (rule ballI)
+                apply (rule ballI)
+                apply (rule impI)
+                apply (drule IHs)
+                apply (erule allE)
+                apply (erule impE)
+                 apply assumption
+                apply assumption
+        (* END REPEAT_DETERM *)
+               apply (rule supp_id_bound bij_id | assumption)+
+      done
+    done
 
+  show "alpha_term x y \<Longrightarrow> FVars_raw_term x = FVars_raw_term y" by (erule x[THEN spec, THEN mp])
+qed
 
+lemma alpha_syms:
+  fixes x::"'a::var_term_pre raw_term"
+  shows "alpha_term x y \<Longrightarrow> alpha_term y x"
+apply (erule alpha_term.coinduct)
+  apply (erule alpha_term.cases)
+  apply hypsubst
 
+  apply (unfold triv_forall_equality)
+  apply (rule exI)+
+  apply (rule conjI, rule refl)+
+  apply (rule conjI[rotated])+
+            apply (rule iffD1[OF term_pre.mr_rel_flip, rotated -1])
+                  apply (unfold inv_id)
+                  apply (erule term_pre.mr_rel_mono_strong0[rotated -7])
+                      apply (rule ballI, rule refl)+
+                      apply (rule ballI, rule inv_inv_eq[THEN fun_cong, symmetric], assumption)+
+(* REPEAT_DETERM *)
+                        apply (rule ballI)
+                        apply (rule ballI)
+                        apply (rule impI)
+                        apply (rule conversepI)
+                        apply (rule disjI1)
+                        apply (assumption | (erule alpha_bij_eq_invs[THEN iffD1, rotated -1], assumption+))
+      (* repeated *)
+                        apply (rule ballI)
+                        apply (rule ballI)
+                        apply (rule impI)
+                        apply (rule conversepI)
+                        apply (rule disjI1)
+                        apply (assumption | (erule alpha_bij_eq_invs[THEN iffD1, rotated -1], assumption+))
+      (* repeated *)
+                        apply (rule ballI)
+                        apply (rule ballI)
+                        apply (rule impI)
+                        apply (rule conversepI)
+                        apply (rule disjI1)
+                        apply (assumption | (erule alpha_bij_eq_invs[THEN iffD1, rotated -1], assumption+))
+      (* END REPEAT_DETERM *)
+                      apply (unfold inv_inv_eq)
+                      apply (assumption | rule supp_id_bound bij_id bij_imp_bij_inv supp_inv_bound)+
 
+           apply (rule iffD2[OF arg_cong[of _ _ eq_on, THEN fun_cong, THEN fun_cong]])
+            apply (erule term_pre.mr_rel_set[rotated -1])
+             apply (rule supp_id_bound | assumption)+
+           apply (rule eq_on_inv2)
+          apply assumption+
 
+          apply (rule id_on_inv)
+        apply assumption+
+       apply (rule id_on_antimono)
+        apply assumption
+       apply (rule equalityD1)
+       apply (rule trans)
+        apply (rule arg_cong2[of _ _ _ _ minus, rotated])
+         apply (rule trans)
+          apply (erule term_pre.mr_rel_set[rotated -1], (rule supp_id_bound bij_id | assumption)+)+
+         apply (rule sym)
+         apply (erule eq_on_image)
+        prefer 2
+        apply (rule trans)
+         apply (rule image_set_diff[OF bij_is_inj, symmetric])
+         apply assumption
+        apply (erule id_on_image)
+       apply (unfold image_UN)[1]
+       apply (rule sym)
+       apply (rule rel_set_UN_D)
+       apply (erule term_pre.mr_set_transfer[THEN rel_funD, rotated -1, OF term_pre.mr_rel_mono_strong[rotated -4]])
+        (* REPEAT_DETERM *)
+                   apply (rule ballI, rule ballI, rule imp_refl)+
+        (* ORELSE *)
+                  apply (rule ballI)
+                  apply (rule ballI)
+                  apply (rule impI)
+                  apply (drule alpha_FVars)
+                  apply (erule trans[rotated])
+                  apply (rule sym)
+                  apply (rule FVars_raw_permutes)
+                   apply assumption+
+            (* ORELSE *)
+                   apply (rule ballI, rule ballI, rule imp_refl)+
+        (* END REPEAT_DETERM *)
+                apply (rule supp_id_bound bij_id supp_inv_bound bij_imp_bij_inv | assumption)+
 
+  apply (rule id_on_inv)
+        apply assumption+
+       apply (rule id_on_antimono)
+        apply assumption
+       apply (rule equalityD1)
+       apply (rule trans)
+     apply (rule arg_cong2[of _ _ _ _ minus, rotated])
+       apply (rule arg_cong2[of _ _ _ _ "(\<union>)"])
+       apply (erule term_pre.mr_rel_set[rotated -1], (rule supp_id_bound bij_id | assumption)+)+
+     prefer 2
+      apply (unfold image_Un[symmetric])[1]
+        apply (rule trans)
+         apply (rule image_set_diff[OF bij_is_inj, symmetric])
+         apply assumption
+        apply (erule id_on_image)
+       apply (unfold image_UN)[1]
+       apply (rule sym)
+       apply (rule rel_set_UN_D)
+       apply (erule term_pre.mr_set_transfer[THEN rel_funD, rotated -1, OF term_pre.mr_rel_mono_strong[rotated -4]])
+        (* REPEAT_DETERM *)
+                  apply (rule ballI)
+                  apply (rule ballI)
+                  apply (rule impI)
+                  apply (drule alpha_FVars)
+                  apply (erule trans[rotated])
+                  apply (rule sym)
+                  apply (rule FVars_raw_permutes)
+                   apply assumption+
+            (* ORELSE *)
+                   apply (rule ballI, rule ballI, rule imp_refl)+
+        (* END REPEAT_DETERM *)
+                apply (rule supp_id_bound bij_id supp_inv_bound bij_imp_bij_inv | assumption)+
+  done
 
+lemma alpha_trans: "alpha_term x y \<Longrightarrow> alpha_term y z \<Longrightarrow> alpha_term x z"
+proof -
+  have x: "(\<exists>y. alpha_term x y \<and> alpha_term y z) \<Longrightarrow> alpha_term x z"
+    apply (erule alpha_term.coinduct)
+    apply (erule exE conjE alpha_term.cases)+
+    apply hypsubst
+    apply (drule iffD1[OF raw_term.inject])
+    apply hypsubst
+    apply (frule term_pre.mr_rel_OO[THEN fun_cong, THEN fun_cong, THEN iffD2, rotated -1, OF relcomppI])
+               apply assumption
+              apply (rule supp_id_bound bij_id | assumption)+
+    apply (unfold id_o o_id)
 
+    apply (unfold triv_forall_equality)
+    subgoal for g x f2 g' y f2' z
+      apply (rule exI[of _ "g' \<circ> g"])
+      apply (rule exI)
+      apply (rule exI[of _ "f2' \<circ> f2"])
+      apply (rule exI)
+      apply (rule conjI, rule refl)+
+      apply (rule conjI, (rule bij_comp supp_comp_bound infinite_UNIV | assumption)+)+
 
+      apply (rule conjI)
+       apply (rule id_on_comp[rotated])
+        apply assumption
+       apply (erule id_on_antimono)
+       apply (rule equalityD2)
+       apply (rule trans)
+        apply (rule arg_cong2[of _ _ _ _ minus, rotated])
+        apply (rule arg_cong2[of _ _ _ _ "(\<union>)"])
+         apply (erule term_pre.mr_rel_set[rotated -1], (rule supp_id_bound bij_id | assumption)+)+
+        prefer 2
+        apply (unfold image_Un[symmetric])
+        apply (rule trans)
+         apply (rule image_set_diff[symmetric, OF bij_is_inj])
+         apply assumption
+        apply (erule id_on_image)
+       apply (unfold image_UN)
+      apply (rule sym)
+       apply (rule rel_set_UN_D)
+       apply (erule term_pre.mr_set_transfer[THEN rel_funD, rotated -1, OF term_pre.mr_rel_mono_strong[rotated -4]])
+        (* REPEAT_DETERM *)
+                   apply (rule ballI)
+                   apply (rule ballI)
+                   apply (rule impI)
+                   apply (drule alpha_FVars)
+                   apply (erule trans[rotated])
+                   apply (rule sym)
+                   apply (rule FVars_raw_permutes)
+                    apply assumption+
+            (* ORELSE *)
+                  apply (rule ballI, rule ballI, rule imp_refl)+
+        (* END REPEAT_DETERM *)
+                apply (rule supp_id_bound bij_id | assumption)+
 
-  
+      apply (rule conjI, (rule bij_comp supp_comp_bound infinite_UNIV | assumption)+)+
+
+            apply (rule conjI)
+       apply (rule id_on_comp[rotated])
+        apply assumption
+       apply (erule id_on_antimono)
+       apply (rule equalityD2)
+       apply (rule trans)
+        apply (rule arg_cong2[of _ _ _ _ minus, rotated])
+        apply (rule trans)
+         apply (erule term_pre.mr_rel_set[rotated -1], (rule supp_id_bound bij_id | assumption)+)+
+        apply (rule sym)
+         apply (erule eq_on_image)
+        prefer 2
+        apply (rule trans)
+         apply (rule image_set_diff[symmetric, OF bij_is_inj])
+         apply assumption
+        apply (erule id_on_image)
+       apply (unfold image_UN)
+      apply (rule sym)
+       apply (rule rel_set_UN_D)
+       apply (erule term_pre.mr_set_transfer[THEN rel_funD, rotated -1, OF term_pre.mr_rel_mono_strong[rotated -4]])
+        (* REPEAT_DETERM *)
+                   apply (rule ballI, rule ballI, rule imp_refl)+
+        (* ORELSE *)
+                   apply (rule ballI)
+                   apply (rule ballI)
+                   apply (rule impI)
+                   apply (drule alpha_FVars)
+                   apply (erule trans[rotated])
+                   apply (rule sym)
+                   apply (rule FVars_raw_permutes)
+                    apply assumption+
+            (* ORELSE *)
+                  apply (rule ballI, rule ballI, rule imp_refl)+
+        (* END REPEAT_DETERM *)
+                apply (rule supp_id_bound bij_id | assumption)+
+
+      apply (rule conjI)
+       apply (rule eq_on_comp)
+        apply (erule eq_on_mono[rotated])
+        apply (rule equalityD1)
+        apply (rule trans)
+         apply (erule eq_on_image)
+        apply (rule sym)
+         apply (erule term_pre.mr_rel_set[rotated -1], (rule supp_id_bound | assumption)+)+
+
+      apply (erule term_pre.mr_rel_mono_strong[rotated -4])
+    (* REPEAT_DETERM *)
+                     apply (rule ballI)
+                     apply (rule ballI)
+                     apply (rule impI)
+                     apply (rule disjI1)
+                     apply (erule relcomppE)
+                     apply (rule exI)
+                     apply (rule conjI[rotated])
+              apply assumption
+             apply (subst permute_raw_comps[symmetric])
+                 apply assumption+
+             apply (rule iffD2[OF alpha_bij_eqs])
+               apply assumption+
+      (* repeated *)
+                     apply (rule ballI)
+                     apply (rule ballI)
+                     apply (rule impI)
+                     apply (rule disjI1)
+                     apply (erule relcomppE)
+                     apply (rule exI)
+                     apply (rule conjI[rotated])
+              apply assumption
+             apply (subst permute_raw_comps[symmetric])
+                 apply assumption+
+             apply (rule iffD2[OF alpha_bij_eqs])
+               apply assumption+
+      (* repeated, free rec case *)
+      apply (rule ballI)
+           apply (rule ballI)
+           apply (rule impI)
+           apply (erule relcomppE)
+           apply (rule disjI1)
+           apply (rule exI)
+           apply (rule conjI)
+            apply assumption+
+      (* END REPEAT_DETERM *)
+          apply (rule supp_id_bound bij_comp supp_comp_bound infinite_UNIV | assumption)+
+      done
+    done
+
+  show "alpha_term x y \<Longrightarrow> alpha_term y z \<Longrightarrow> alpha_term x z"
+    apply (rule x)
+    apply (rule exI)
+    apply (rule conjI)
+     apply assumption+
+    done
+qed
+
+lemma raw_refreshs:
+  fixes x::"('a::var_term_pre, 'a, 'a, 'a raw_term, 'a raw_term, 'a raw_term) term_pre"
+  assumes "|A| <o |UNIV::'a set|"
+  shows "\<exists>y. (set2_term_pre y \<union> set3_term_pre y) \<inter> A = {} \<and> alpha_term (raw_term_ctor x) (raw_term_ctor y)"
+
+  apply (rule exE[OF eextend_fresh[of "set2_term_pre x \<union> set3_term_pre x"
+    "(A \<union> (set2_term_pre x \<union> set3_term_pre x)) \<union> ((\<Union>(FVars_raw_term ` set4_term_pre x) \<union> \<Union>(FVars_raw_term ` set5_term_pre x)) - (set2_term_pre x \<union> set3_term_pre x))"
+    "(\<Union>(FVars_raw_term ` set4_term_pre x) \<union> \<Union>(FVars_raw_term ` set5_term_pre x)) - (set2_term_pre x \<union> set3_term_pre x)"
+  ]])
+       apply (rule var_term_pre_class.Un_bound term_pre.set_bd_UNIV assms ordLeq_ordLess_trans[OF card_of_diff]
+        term_pre.set_bd[THEN ordLess_ordLeq_trans] var_term_pre_class.UN_bound var_term_pre_class.large FVars_raw_bd_UNIVs infinite_UNIV
+      )+
+    apply (rule Un_upper2)
+   apply (rule Diff_disjoint)
+  apply (erule conjE)+
+  apply (unfold Un_Diff)
+
+  subgoal for g
+    apply (rule exE[OF extend_id_on[of g "\<Union> (FVars_raw_term ` set5_term_pre x)" "set2_term_pre x \<union> set3_term_pre x" "set3_term_pre x"]])
+          apply assumption+
+        apply (erule id_on_antimono)
+        apply (rule Un_upper2)
+       apply assumption
+      apply (erule Int_subset_empty2)
+      apply (rule subset_trans[rotated])
+       apply (rule Un_upper1)
+      apply (rule Un_upper2)
+
+     apply (rule subsetI)
+     apply (rotate_tac -1)
+     apply (erule contrapos_pp)
+     apply (unfold Un_iff de_Morgan_disj)[1]
+     apply (erule conjE)+
+     apply assumption
+    apply (erule conjE)+
+
+    subgoal for f2
+      apply (rule exI[of _ "map_term_pre id g g (permute_raw_term g) (permute_raw_term f2) id x"])
+      apply (subst term_pre.set_map, (rule supp_id_bound bij_id | assumption)+)+
+      apply (unfold image_Un[symmetric])
+      apply (rule conjI)
+       apply (erule Int_subset_empty2)
+       apply (unfold Un_assoc)[1]
+       apply (rule Un_upper1)
+      apply (rule alpha_term.intros[rotated -1])
+                apply (rule iffD2[OF term_pre.mr_rel_map(3), rotated -1])
+                          apply (unfold inv_id id_o Grp_UNIV_id conversep_eq OO_eq)
+                          apply (subst inv_o_simp1, assumption)+
+                          apply (unfold term_pre.mr_rel_id[symmetric] relcompp_conversep_Grp)
+                          apply (rule term_pre.rel_refl_strong)
+                          apply (rule alpha_refls)+
+                          apply (rule supp_id_bound bij_id | assumption)+
+
+           apply (erule id_on_antimono)
+           apply (rule Un_upper1)
+         apply assumption+
+      done
+    done
+  done
+
+lemma avoid_raw_freshs:
+  fixes x::"'a::var_term_pre raw_term_pre"
+  assumes "|A| <o |UNIV::'a set|"
+shows "set2_term_pre (avoid_raw_term x A) \<inter> A = {}" "set3_term_pre (avoid_raw_term x A) \<inter> A = {}"
+   apply (unfold avoid_raw_term_def)
+  (* REPEAT_DETERM *)
+   apply (rule someI2_ex)
+    apply (rule raw_refreshs[OF assms])
+  apply (unfold Int_Un_distrib2 Un_empty)[1]
+   apply (erule conjE)+
+   apply assumption
+  (* repeated *)
+   apply (rule someI2_ex)
+    apply (rule raw_refreshs[OF assms])
+  apply (unfold Int_Un_distrib2 Un_empty)[1]
+   apply (erule conjE)+
+   apply assumption
+  (* END REPEAT_DETERM *)
+  done
+
+lemma TT_Quotients: "Quotient alpha_term TT_abs TT_rep (\<lambda>x. (=) (TT_abs x))"
+  apply (subgoal_tac "Quotient3 alpha_term TT_abs TT_rep")
+   prefer 2
+   apply (rule quot_type.Quotient)
+   apply (rule type_definition_quot_type)
+    apply (rule type_definition_term)
+   apply (rule equivpI)
+     apply (rule reflpI)
+     apply (rule alpha_refls)
+    apply (rule sympI)
+    apply (erule alpha_syms)
+   apply (rule transpI)
+   apply (erule alpha_trans)
+   apply assumption
+  apply (rule QuotientI)
+     apply (erule Quotient3_abs_rep)
+    apply (rule alpha_refls)
+   apply (erule Quotient3_rel[symmetric])
+  apply (rule ext)+
+  apply (rule iffI)
+   apply (rule conjI)
+    apply (rule alpha_refls)
+   apply assumption
+  apply (erule conjE)
+  apply assumption
+  done
+
+lemmas TT_total_abs_eq_iffs = TT_Quotients[THEN Quotient_total_abs_eq_iff, OF reflpI[OF alpha_refls]]
+lemmas TT_rep_abs = TT_Quotients[THEN Quotient_rep_abs, OF alpha_refls]
+lemmas TT_abs_rep = TT_Quotients[THEN Quotient_abs_rep]
+
+lemmas TT_rep_abs_syms = alpha_syms[OF TT_rep_abs]
+
+lemma TT_abs_ctors: "TT_abs (raw_term_ctor x) = term_ctor (map_term_pre id id id TT_abs TT_abs TT_abs x)"
+  apply (unfold term_ctor_def)
+  apply (rule TT_total_abs_eq_iffs[THEN iffD2])
+  apply (rule alpha_term.intros)
+         apply (rule supp_id_bound bij_id id_on_id eq_on_refl)+
+  apply (unfold permute_raw_ids term_pre.mr_rel_id[symmetric])
+  apply (subst term_pre.map_comp)
+    apply (rule supp_id_bound bij_id)+
+  apply (unfold id_o o_id)
+  apply (rule iffD2[OF term_pre.rel_map(2)])
+  apply (unfold comp_def)
+  apply (rule term_pre.rel_refl_strong)
+    apply (rule TT_rep_abs_syms)+
+  done
+
+lemma permute_simps:
+  fixes f::"'a::var_term_pre \<Rightarrow> 'a"
+  assumes "bij f" "|supp f| <o |UNIV::'a set|"
+  shows "permute_term f (term_ctor x) = term_ctor (map_term_pre f f f (permute_term f) (permute_term f) (permute_term f) x)"
+  apply (unfold term_ctor_def permute_term_def)
+  apply (subst term_pre.map_comp)
+      apply (rule supp_id_bound bij_id assms)+
+  apply (unfold id_o o_id)
+  apply (unfold comp_def)
+  apply (rule TT_total_abs_eq_iffs[THEN iffD2])
+  apply (rule alpha_bij_eq_invs[OF assms, THEN iffD2])
+  apply (subst permute_raw_simps)
+    apply (rule bij_imp_bij_inv supp_inv_bound assms)+
+  apply (subst term_pre.map_comp)
+      apply (rule bij_imp_bij_inv supp_inv_bound assms)+
+  apply (subst inv_o_simp1, rule assms)+
+  apply (rule alpha_trans)
+  apply (rule TT_rep_abs)
+  apply (unfold comp_def)
+  apply (rule alpha_term.intros)
+         apply (rule bij_id supp_id_bound id_on_id eq_on_refl)+
+  apply (rule iffD2[OF term_pre.mr_rel_id[symmetric, THEN fun_cong, THEN fun_cong]])
+  apply (rule iffD2[OF term_pre.rel_map(1)])
+  apply (rule iffD2[OF term_pre.rel_map(2)])
+  apply (unfold permute_raw_ids)
+  apply (rule term_pre.rel_refl_strong)
+  (* REPEAT_DETERM *)
+    apply (rule alpha_bij_eq_invs[THEN iffD1])
+      apply (rule assms supp_id_bound bij_id)+
+    apply (rule TT_rep_abs_syms)
+  (* repeated *)
+    apply (rule alpha_bij_eq_invs[THEN iffD1])
+      apply (rule assms supp_id_bound bij_id)+
+    apply (rule TT_rep_abs_syms)
+  (* repeated *)
+    apply (rule alpha_bij_eq_invs[THEN iffD1])
+      apply (rule assms supp_id_bound bij_id)+
+    apply (rule TT_rep_abs_syms)
+  (* END REPEAT_DETERM *)
+  done
+
+lemma permute_ids: "permute_term id x = x"
+  apply (unfold permute_term_def permute_raw_ids TT_abs_rep)
+  apply (rule refl)
+  done
+
+lemmas permute_id0s = permute_ids[THEN trans[OF _ id_apply[symmetric]], abs_def, THEN meta_eq_to_obj_eq]
+
+lemma permute_comps:
+  fixes f::"'a::var_term_pre \<Rightarrow> 'a"
+  assumes "bij f" "|supp f| <o |UNIV::'a set|" "bij g" "|supp g| <o |UNIV::'a set|"
+  shows "permute_term g (permute_term f x) = permute_term (g \<circ> f) x"
+  apply (unfold permute_term_def)
+  apply (subst permute_raw_comps[symmetric])
+      apply (rule assms)+
+  apply (rule TT_total_abs_eq_iffs[THEN iffD2])
+  apply (rule alpha_bij_eqs[THEN iffD2])
+    apply (rule assms)+
+  apply (rule TT_rep_abs)
+  done
+
+lemma permute_comp0s:
+  fixes f::"'a::var_term_pre \<Rightarrow> 'a"
+  assumes "bij f" "|supp f| <o |UNIV::'a set|" "bij g" "|supp g| <o |UNIV::'a set|"
+  shows "permute_term g \<circ> permute_term f = permute_term (g \<circ> f)"
+  apply (rule ext)
+  apply (rule trans[OF comp_apply])
+  apply (rule permute_comps[OF assms])
+  done
+
+lemma permute_bijs:
+  fixes f::"'a::var_term_pre \<Rightarrow> 'a"
+  assumes "bij f" "|supp f| <o |UNIV::'a set|"
+  shows "bij (permute_term f)"
+  apply (rule o_bij)
+   apply (rule trans)
+    apply (rule permute_comp0s)
+       prefer 5 (* 4 * nvars + 1 *)
+       apply (subst inv_o_simp1, rule assms)+
+       apply (rule permute_id0s)
+      apply (rule bij_imp_bij_inv supp_inv_bound assms)+
+  apply (rule trans)
+   apply (rule permute_comp0s)
+      apply (rule bij_imp_bij_inv supp_inv_bound assms)+
+  apply (subst inv_o_simp2, rule assms)+
+  apply (rule permute_id0s)
+  done
+
+lemma permute_inv_simps:
+  fixes f::"'a::var_term_pre \<Rightarrow> 'a"
+  assumes "bij f" "|supp f| <o |UNIV::'a set|"
+  shows "inv (permute_term f) = permute_term (inv f)"
+  apply (rule inv_unique_comp)
+  (* REPEAT_DETERM *)
+   apply (rule trans)
+    apply (rule permute_comp0s)
+       apply (rule bij_imp_bij_inv supp_inv_bound assms)+
+   apply (subst inv_o_simp1 inv_o_simp2, rule assms)+
+   apply (rule permute_id0s)
+  (* repeated *)
+   apply (rule trans)
+    apply (rule permute_comp0s)
+       apply (rule bij_imp_bij_inv supp_inv_bound assms)+
+   apply (subst inv_o_simp1 inv_o_simp2, rule assms)+
+  apply (rule permute_id0s)
+  done
+
+lemma FVars_bds: "|FVars_term x| <o natLeq"
+  apply (unfold FVars_term_def)
+  apply (rule FVars_raw_bds)
+  done
+
+lemmas FVars_bd_UNIVs = ordLess_ordLeq_trans[OF FVars_bds var_term_pre_class.large]
+
+lemma FVars_permutes:
+  fixes f::"'a::var_term_pre \<Rightarrow> 'a"
+  assumes "bij f" "|supp f| <o |UNIV::'a set|"
+  shows "FVars_term (permute_term f x) = f ` FVars_term x"
+  apply (unfold FVars_term_def permute_term_def)
+  apply (rule trans)
+   apply (rule alpha_FVars)
+   apply (rule TT_rep_abs)
+  apply (rule FVars_raw_permutes[OF assms])
+  done
+
+lemma FVars_ctors:
+  "FVars_term (term_ctor x) = set1_term_pre x \<union> (\<Union>(FVars_term ` set4_term_pre x) - (set2_term_pre x \<union> set3_term_pre x))
+   \<union> (\<Union>(FVars_term ` set5_term_pre x) - set3_term_pre x) \<union> \<Union>(FVars_term ` set6_term_pre x)"
+  apply (unfold FVars_term_def term_ctor_def)
+  apply (rule trans)
+   apply (rule alpha_FVars)
+   apply (rule TT_rep_abs)
+  apply (rule trans)
+   apply (rule FVars_raw_ctors)
+  apply (subst term_pre.set_map, (rule supp_id_bound bij_id)+)+
+  apply (unfold image_id image_comp[unfolded comp_def])
+  apply (rule refl)
+  done
+
+lemma FVars_intros:
+  "a \<in> set1_term_pre x \<Longrightarrow> a \<in> FVars_term (term_ctor x)"
+  "z \<in> set4_term_pre x \<Longrightarrow> a \<in> FVars_term z \<Longrightarrow> a \<notin> set2_term_pre x \<union> set3_term_pre x \<Longrightarrow> a \<in> FVars_term (term_ctor x)"
+  "z \<in> set5_term_pre x \<Longrightarrow> a \<in> FVars_term z \<Longrightarrow> a \<notin> set3_term_pre x \<Longrightarrow> a \<in> FVars_term (term_ctor x)"
+  "z \<in> set6_term_pre x \<Longrightarrow> a \<in> FVars_term z \<Longrightarrow> a \<in> FVars_term (term_ctor x)"
+     apply (unfold FVars_term_def term_ctor_def alpha_FVars[OF TT_rep_abs])
+  (* for thm in FVars_intros *)
+     apply (drule iffD1[OF arg_cong2[OF refl, of _ _ "(\<in>)"], rotated -1])
+      prefer 2
+      apply (erule FVars_raw_intros(1)[rotated])
+     apply (subst term_pre.set_map)
+       apply (rule supp_id_bound bij_id)+
+     apply (unfold image_id)?
+     apply assumption?
+     apply (subst term_pre.set_map, (rule supp_id_bound bij_id)+)?
+     apply (erule imageI)?
+     apply (rule refl)
+  (* repeated *)
+     apply (drule iffD1[OF arg_cong2[OF refl, of _ _ "(\<in>)"], rotated -1])
+      prefer 2
+      apply (erule FVars_raw_intros(2)[rotated])
+     apply (subst term_pre.set_map, (rule supp_id_bound bij_id)+)+
+     apply (unfold image_id)?
+     apply assumption?
+     apply (subst term_pre.set_map, (rule supp_id_bound bij_id)+)?
+     apply (erule imageI)?
+     apply (rule refl)
+  (* repeated *)
+     apply (drule iffD1[OF arg_cong2[OF refl, of _ _ "(\<in>)"], rotated -1])
+      prefer 2
+      apply (erule FVars_raw_intros(3)[rotated])
+     apply (subst term_pre.set_map, (rule supp_id_bound bij_id)+)+
+     apply (unfold image_id)?
+     apply assumption?
+     apply (subst term_pre.set_map, (rule supp_id_bound bij_id)+)?
+     apply (erule imageI)?
+     apply (rule refl)
+  (* repeated *)
+     apply (drule iffD1[OF arg_cong2[OF refl, of _ _ "(\<in>)"], rotated -1])
+      prefer 2
+      apply (erule FVars_raw_intros(4)[rotated])
+     apply (subst term_pre.set_map, (rule supp_id_bound bij_id)+)+
+     apply (unfold image_id)?
+     apply assumption?
+     apply (subst term_pre.set_map, (rule supp_id_bound bij_id)+)?
+     apply (erule imageI)?
+     apply (rule refl)
+  (* END REPEAT_DETERM *)
+  done
+
+lemma TT_inject0s:
+  "(term_ctor x = term_ctor y) \<longleftrightarrow> (\<exists>(g::'a::var_term_pre \<Rightarrow> 'a) f2.
+    bij g \<and> |supp g| <o |UNIV::'a set| \<and>
+    id_on (\<Union>(FVars_term ` set4_term_pre x) - (set2_term_pre x \<union> set3_term_pre x)) g \<and>
+    bij f2 \<and> |supp f2| <o |UNIV::'a set| \<and> id_on (\<Union>(FVars_term ` set5_term_pre x) - set3_term_pre x) f2 \<and>
+    eq_on (set3_term_pre x) f2 g \<and>
+    map_term_pre id g g (permute_term g) (permute_term f2) id x = y)"
+  apply (unfold term_ctor_def permute_term_def)
+  apply (rule trans)
+   apply (rule TT_total_abs_eq_iffs)
+  apply (rule iffI)
+   apply (erule alpha_term.cases)
+   apply (drule iffD1[OF raw_term.inject])+
+   apply hypsubst
+   apply (subst (asm) term_pre.set_map, (rule supp_id_bound bij_id)+)+
+   apply (unfold image_id image_comp[unfolded comp_def])
+   apply (drule iffD1[OF term_pre.mr_rel_map(1), rotated -1])
+             apply (rule supp_id_bound bij_id | assumption)+
+   apply (unfold id_o o_id)
+   apply (drule iffD1[OF term_pre.mr_rel_map(3), rotated -1])
+              apply (rule supp_id_bound bij_id | assumption)+
+   apply (unfold inv_id id_o o_id relcompp_conversep_Grp)
+   apply (unfold Grp_OO FVars_term_def[symmetric])
+   apply (rule exI)+
+   apply (rule conjI[rotated])+
+          apply (rule term_pre.mr_rel_eq[THEN fun_cong, THEN fun_cong, THEN iffD1])
+          apply (rule iffD2[OF term_pre.mr_rel_map(1), rotated -1])
+                    apply (unfold id_o o_id Grp_OO)
+                    apply (erule term_pre.mr_rel_mono_strong[rotated -4])
+            (* REPEAT_DETERM *)
+                      apply (rule ballI impI)+
+                      apply (drule TT_total_abs_eq_iffs[THEN iffD2])
+                      apply (unfold TT_abs_rep)
+                      apply assumption
+            (* repeated *)
+                      apply (rule ballI impI)+
+                      apply (drule TT_total_abs_eq_iffs[THEN iffD2])
+                      apply (unfold TT_abs_rep)
+                      apply assumption
+            (* repeated *)
+                      apply (rule ballI impI)+
+                      apply (drule TT_total_abs_eq_iffs[THEN iffD2])
+                      apply (unfold TT_abs_rep)
+                      apply hypsubst
+                      apply (rule id_apply)
+            (* END REPEAT_DETERM *)
+                      apply (rule supp_id_bound bij_id | assumption)+
+
+  apply (erule exE conjE)+
+  apply hypsubst_thin
+  apply (subst term_pre.map_comp)
+      apply (rule supp_id_bound bij_id | assumption)+
+  apply (unfold id_o o_id)
+  apply (unfold comp_def)
+  apply (rule alpha_term.intros[rotated -1])
+         apply (rule iffD2[OF term_pre.mr_rel_map(1), rotated -1])
+                   apply (unfold id_o o_id Grp_UNIV_id eq_OO)
+                   apply (rule iffD2[OF term_pre.mr_rel_map(3), rotated -1])
+                      apply (unfold inv_id id_o o_id Grp_UNIV_id conversep_eq eq_OO)
+                      apply (unfold relcompp_conversep_Grp Grp_OO)
+                      apply (subst inv_o_simp1, assumption)+
+                      apply (rule iffD1[OF term_pre.mr_rel_id[THEN fun_cong, THEN fun_cong]])
+                      apply (rule term_pre.rel_refl_strong)
+                      apply (rule alpha_refls TT_rep_abs_syms)+
+                      apply (rule supp_id_bound bij_id | assumption)+
+              (* REPEAT_DETERM *)
+      apply (subst term_pre.set_map, (rule supp_id_bound bij_id)+)+
+      apply (unfold image_id FVars_term_def image_comp[unfolded comp_def])
+      apply assumption+
+      (* repeated *)
+      apply (subst term_pre.set_map, (rule supp_id_bound bij_id)+)+
+      apply (unfold image_id FVars_term_def image_comp[unfolded comp_def])
+      apply assumption+
+      (* repeated *)
+      apply (subst term_pre.set_map, (rule supp_id_bound bij_id)+)+
+      apply (unfold image_id FVars_term_def image_comp[unfolded comp_def])
+      apply assumption+
+      (* END REPEAT_DETERM *)
+  done
+
+lemma avoid_freshs:
+  fixes x::"'a::var_term_pre term_pre'"
+  assumes "|A| <o |UNIV::'a set|"
+  shows "set2_term_pre (avoid_term x A) \<inter> A = {}" "set3_term_pre (avoid_term x A) \<inter> A = {}"
+   apply (unfold avoid_term_def)
+  (* REPEAT_DETERM *)
+   apply (subst term_pre.set_map, (rule supp_id_bound bij_id)+)+
+   apply (unfold image_id)
+   apply (rule avoid_raw_freshs[OF assms])
+   (* repeated *)
+   apply (subst term_pre.set_map, (rule supp_id_bound bij_id)+)+
+   apply (unfold image_id)
+   apply (rule avoid_raw_freshs[OF assms])
+   (* END REPEAT_DETERM *)
+  done
+
+lemma alpha_avoids:
+  fixes x::"'a::var_term_pre term_pre'"
+  assumes "|A| <o |UNIV::'a set|"
+  shows "term_ctor (avoid_term x A) = term_ctor x"
+  apply (unfold avoid_term_def avoid_raw_term_def)
+  apply (rule someI2_ex)
+   apply (rule raw_refreshs[OF assms])
+  apply (erule conjE)+
+  apply (unfold term_ctor_def)
+  apply (subst term_pre.map_comp)
+    apply (rule supp_id_bound bij_id)+
+  apply (unfold id_o o_id)
+  apply (drule TT_total_abs_eq_iffs[THEN iffD2])
+  apply (rule trans[rotated])
+   apply (erule sym)
+  apply (rule TT_total_abs_eq_iffs[THEN iffD2])
+  apply (rule alpha_term.intros)
+         apply (rule supp_id_bound bij_id id_on_id eq_on_refl)+
+  apply (rule iffD2[OF term_pre.mr_rel_map(1), rotated -1])
+            apply (unfold id_o o_id Grp_OO permute_raw_ids)
+            apply (unfold comp_def term_pre.mr_rel_id[symmetric])
+            apply (rule term_pre.rel_refl_strong)
+              apply (rule TT_rep_abs)+
+           apply (rule supp_id_bound bij_id)+
+  done
+
+lemma fresh_cases:
+  fixes y::"'a::var_term_pre term"
+  assumes "|A| <o |UNIV::'a set|"
+  and "\<And>(x::'a term_pre'). y = term_ctor x \<Longrightarrow> set2_term_pre x \<inter> A = {} \<Longrightarrow> set3_term_pre x \<inter> A = {} \<Longrightarrow> P"
+shows P
+  apply (rule raw_term.exhaust[of "TT_rep y"])
+  apply (rule assms)
+    defer
+    apply (rule avoid_freshs[OF assms(1)])+
+  apply (rule trans[rotated])
+   apply (rule sym)
+   apply (rule alpha_avoids[OF assms(1)])
+  apply (unfold term_ctor_def)
+  apply (rule TT_Quotients[THEN Quotient_rel_abs2])
+  apply (rule arg_cong2[OF _ refl, of _ _ alpha_term, THEN iffD2])
+   apply assumption
+  apply (rule alpha_term.intros)
+         apply (rule supp_id_bound bij_id id_on_id eq_on_refl)+
+         apply (subst term_pre.map_comp)
+                apply (rule supp_id_bound bij_id)+
+         apply (unfold id_o o_id)
+         apply (rule iffD2[OF term_pre.mr_rel_map(3), rotated -1])
+                    apply (unfold inv_id id_o o_id Grp_OO relcompp_conversep_Grp)
+             apply (unfold comp_def term_pre.mr_rel_id[symmetric] permute_raw_ids)
+             apply (rule term_pre.rel_refl_strong)
+               apply (rule TT_rep_abs_syms)+
+            apply (rule supp_id_bound bij_id)+
+  done
+
+lemma alpha_subshapess: "alpha_term x y \<Longrightarrow> subshape_term_term z x \<Longrightarrow> subshape_term_term z y"
+proof -
+  have x: "(\<forall>x. alpha_term x y \<longrightarrow> (\<forall>z. subshape_term_term z x \<longrightarrow> subshape_term_term z y))"
+    apply (rule raw_term.induct[of _ y])
+    subgoal premises IHs for x
+      apply (rule allI impI)+
+      apply (erule alpha_term.cases)
+      apply (erule subshape_term_term.cases)
+      apply hypsubst
+      apply (drule iffD1[OF raw_term.inject])+
+      apply hypsubst
+      apply (erule UnE)+
+    (* REPEAT_DETERM *)
+        apply (drule term_pre.mr_rel_set(4-6)[rotated -1])
+              prefer 6 (* free + 2 * bound + 1 *)
+              apply assumption
+             apply (rule supp_id_bound bij_id | assumption)+
+        apply (erule bexE)
+        apply (frule IHs)
+        apply (erule allE)
+        apply (erule impE)
+         apply assumption
+        apply (rule subshape_term_term.intros[rotated -1])
+           apply (tactic \<open>eresolve_tac @{context} [BNF_Util.mk_UnIN 3 1] 1\<close>)
+          prefer 3 (* 2 * nvars + 1 *)
+          apply (rule alpha_trans[rotated])
+           apply assumption
+          apply (rule alpha_trans[rotated])
+           apply (rule alpha_bij_eqs[THEN iffD2, rotated -1])
+             apply assumption+
+          apply (rule iffD2[OF arg_cong2[OF _ refl, of _ _ alpha_term], rotated])
+           apply (rule alpha_refls)
+          apply (rule sym)
+          apply (rule permute_raw_comps)
+             apply assumption+
+         apply (rule bij_comp supp_comp_bound infinite_UNIV | assumption)+
+      (* repeated *)
+        apply (drule term_pre.mr_rel_set(4-6)[rotated -1])
+              prefer 6 (* free + 2 * bound + 1 *)
+              apply assumption
+             apply (rule supp_id_bound bij_id | assumption)+
+        apply (erule bexE)
+        apply (frule IHs)
+        apply (erule allE)
+        apply (erule impE)
+         apply assumption
+        apply (rule subshape_term_term.intros[rotated -1])
+           apply (tactic \<open>eresolve_tac @{context} [BNF_Util.mk_UnIN 3 2] 1\<close>)
+          prefer 3 (* 2 * nvars + 1 *)
+          apply (rule alpha_trans[rotated])
+           apply assumption
+          apply (rule alpha_trans[rotated])
+           apply (rule alpha_bij_eqs[THEN iffD2, rotated -1])
+             apply assumption+
+          apply (rule iffD2[OF arg_cong2[OF _ refl, of _ _ alpha_term], rotated])
+           apply (rule alpha_refls)
+          apply (rule sym)
+          apply (rule permute_raw_comps)
+             apply assumption+
+        apply (rule bij_comp supp_comp_bound infinite_UNIV | assumption)+
+        (* repeated *)
+        apply (drule term_pre.mr_rel_set(4-6)[rotated -1])
+              prefer 6 (* free + 2 * bound + 1 *)
+              apply assumption
+             apply (rule supp_id_bound bij_id | assumption)+
+        apply (erule bexE)
+        apply (frule IHs)
+        apply (erule allE)
+        apply (erule impE)
+         apply assumption
+        apply (rule subshape_term_term.intros[rotated -1])
+           apply (tactic \<open>eresolve_tac @{context} [BNF_Util.mk_UnIN 3 3] 1\<close>)
+          prefer 3 (* 2 * nvars + 1 *)
+          apply (rule alpha_trans[rotated])
+         apply assumption+
+      (* END REPEAT_DETERM *)
+      done
+    done
+
+  show "alpha_term x y \<Longrightarrow> subshape_term_term z x \<Longrightarrow> subshape_term_term z y"
+    apply (erule x[THEN spec, THEN mp, THEN spec, THEN mp])
+    apply assumption
+    done
+qed
+
+lemma subshape_induct_raw:
+  fixes x::"'a::var_term_pre raw_term"
+  assumes "\<And>x. (\<And>y. subshape_term_term y x \<Longrightarrow> P y) \<Longrightarrow> P x"
+  shows "\<forall>f y. bij f \<longrightarrow> |supp f| <o |UNIV::'a set| \<longrightarrow> alpha_term (permute_raw_term f x) y \<longrightarrow> P y"
+  apply (rule raw_term.induct[of _ x])
+  subgoal premises IHs for x
+    apply (rule allI impI)+
+    apply (rule assms)
+    (* REPEAT_DETERM *)
+    apply (drule alpha_subshapess[rotated -1])
+     apply (erule alpha_syms)
+    apply (rotate_tac -2)
+    apply (erule thin_rl)
+    apply (subst (asm) permute_raw_simps)
+      apply assumption+
+    apply (erule subshape_term_term.cases)
+    apply (drule iffD1[OF raw_term.inject])
+    apply hypsubst
+    apply (subst (asm) term_pre.set_map, (assumption | rule supp_id_bound bij_id)+)+
+    apply (unfold image_Un[symmetric])
+    apply (erule imageE)
+    apply hypsubst
+    apply (drule alpha_bij_eq_invs[THEN iffD1, rotated -1])
+      apply assumption+
+    apply (subst (asm) permute_raw_comps)
+        apply (assumption | rule bij_imp_bij_inv supp_inv_bound)+
+    apply (erule UnE)+
+  (* REPEAT_DETERM *)
+      apply (drule IHs)
+      apply (erule allE)+
+    (* REPEAT_DETERM *)
+      apply (erule impE) prefer 2
+    apply (erule impE) prefer 2
+    apply (erule impE) prefer 2
+  (* END REPEAT_DETERM *)
+         apply assumption
+        apply (erule alpha_syms)
+       apply (assumption | rule bij_imp_bij_inv supp_inv_bound supp_comp_bound bij_comp infinite_UNIV)+
+    (* repeated *)
+      apply (drule IHs)
+      apply (erule allE)+
+    (* REPEAT_DETERM *)
+      apply (erule impE) prefer 2
+    apply (erule impE) prefer 2
+    apply (erule impE) prefer 2
+  (* END REPEAT_DETERM *)
+         apply assumption
+        apply (erule alpha_syms)
+       apply (assumption | rule bij_imp_bij_inv supp_inv_bound supp_comp_bound bij_comp infinite_UNIV)+
+    (* repeated *)
+      apply (drule IHs)
+      apply (erule allE)+
+    (* REPEAT_DETERM *)
+      apply (erule impE) prefer 2
+    apply (erule impE) prefer 2
+    apply (erule impE) prefer 2
+  (* END REPEAT_DETERM *)
+         apply assumption
+        apply (erule alpha_syms)
+       apply (assumption | rule bij_imp_bij_inv supp_inv_bound supp_comp_bound bij_comp infinite_UNIV)+
+    (* END REPEAT_DETERM *)
+    done
+  done
+
+lemma subshape_induct:
+  fixes x::"'a::var_term_pre raw_term"
+  assumes "\<And>x. (\<And>y. subshape_term_term y x \<Longrightarrow> P y) \<Longrightarrow> P x"
+  shows "P x"
+  apply (rule subshape_induct_raw[THEN spec, THEN spec, THEN mp, THEN mp, THEN mp])
+     apply (rule assms)
+     apply assumption
+    apply (rule bij_id supp_id_bound)+
+  apply (unfold permute_raw_ids)
+  apply (rule alpha_refls)
+  done
+
+lemma wf_subshape: "wf {(x, y). subshape_term_term x y }"
+  apply (rule wfUNIVI)
+  apply (unfold prod_in_Collect_iff prod.case)
+    apply (rule subshape_induct)
+    apply (erule allE)
+    apply (erule impE)
+    apply (rule allI)
+     apply (rule impI)
+     apply assumption
+    apply assumption
+  done
+
+lemma set_subshapess:
+  "z \<in> set4_term_pre x \<Longrightarrow> subshape_term_term z (raw_term_ctor x)"
+  "z \<in> set5_term_pre x \<Longrightarrow> subshape_term_term z (raw_term_ctor x)"
+  "z \<in> set6_term_pre x \<Longrightarrow> subshape_term_term z (raw_term_ctor x)"
+  (* REPEAT_DETERM *)
+    apply (rule subshape_term_term.intros)
+       apply (rule supp_id_bound bij_id)+
+     apply (unfold permute_raw_ids)
+     apply (rule alpha_refls)
+    apply (tactic \<open>eresolve_tac @{context} [BNF_Util.mk_UnIN 3 1] 1\<close>)
+  (* repeated *)
+    apply (rule subshape_term_term.intros)
+       apply (rule supp_id_bound bij_id)+
+     apply (unfold permute_raw_ids)
+     apply (rule alpha_refls)
+    apply (tactic \<open>eresolve_tac @{context} [BNF_Util.mk_UnIN 3 2] 1\<close>)
+  (* repeated *)
+    apply (rule subshape_term_term.intros)
+       apply (rule supp_id_bound bij_id)+
+     apply (unfold permute_raw_ids)
+     apply (rule alpha_refls)
+    apply (tactic \<open>eresolve_tac @{context} [BNF_Util.mk_UnIN 3 3] 1\<close>)
+  (* END REPEAT_DETERM *)
+  done
+
+lemma set_subshape_permutess:
+  fixes f::"'a::var_term_pre \<Rightarrow> 'a"
+  assumes "bij f" "|supp f| <o |UNIV::'a set|"
+  shows
+  "z \<in> set4_term_pre x \<Longrightarrow> subshape_term_term (permute_raw_term f z) (raw_term_ctor x)"
+  "z \<in> set5_term_pre x \<Longrightarrow> subshape_term_term (permute_raw_term f z) (raw_term_ctor x)"
+  "z \<in> set6_term_pre x \<Longrightarrow> subshape_term_term (permute_raw_term f z) (raw_term_ctor x)"
+  (* REPEAT_DETERM *)
+    apply (rule subshape_term_term.intros[rotated -2])
+       apply (subst permute_raw_comps)
+           prefer 5 (* 4 * nvars + 1 *)
+           apply (subst inv_o_simp1, rule assms)+
+           apply (unfold permute_raw_ids)
+           apply (rule alpha_refls)
+                     apply (rule assms bij_imp_bij_inv supp_inv_bound)+
+      apply (tactic \<open>eresolve_tac @{context} [BNF_Util.mk_UnIN 3 1] 1\<close>)
+     apply (rule assms bij_imp_bij_inv supp_inv_bound)+
+      (* repeated *)
+    apply (rule subshape_term_term.intros[rotated -2])
+       apply (subst permute_raw_comps)
+           prefer 5 (* 4 * nvars + 1 *)
+           apply (subst inv_o_simp1, rule assms)+
+           apply (unfold permute_raw_ids)
+           apply (rule alpha_refls)
+                     apply (rule assms bij_imp_bij_inv supp_inv_bound)+
+      apply (tactic \<open>eresolve_tac @{context} [BNF_Util.mk_UnIN 3 2] 1\<close>)
+     apply (rule assms bij_imp_bij_inv supp_inv_bound)+
+      (* repeated *)
+    apply (rule subshape_term_term.intros[rotated -2])
+       apply (subst permute_raw_comps)
+           prefer 5 (* 4 * nvars + 1 *)
+           apply (subst inv_o_simp1, rule assms)+
+           apply (unfold permute_raw_ids)
+           apply (rule alpha_refls)
+                     apply (rule assms bij_imp_bij_inv supp_inv_bound)+
+      apply (tactic \<open>eresolve_tac @{context} [BNF_Util.mk_UnIN 3 3] 1\<close>)
+     apply (rule assms bij_imp_bij_inv supp_inv_bound)+
+      (* END REPEAT_DETERM *)
+  done
+
+lemma permute_abs:
+  fixes f::"'a::var_term_pre \<Rightarrow> 'a"
+  assumes "bij f" "|supp f| <o |UNIV::'a set|"
+  shows "permute_term f (TT_abs x) = TT_abs (permute_raw_term f x)"
+  apply (unfold permute_term_def)
+  apply (rule TT_total_abs_eq_iffs[THEN iffD2])
+  apply (rule alpha_bij_eqs[THEN iffD2, OF assms])
+  apply (rule TT_rep_abs)
+  done
+
+lemma permute_congs:
+  fixes f g::"'a::var_term_pre \<Rightarrow> 'a"
+  assumes "bij f" "|supp f| <o |UNIV::'a set|" "bij g" "|supp g| <o |UNIV::'a set|"
+  shows "(\<And>a. a \<in> FVars_term x \<Longrightarrow> f a = g a) \<Longrightarrow> permute_term f x = permute_term g x"
+  apply (unfold permute_term_def atomize_all atomize_imp eq_on_def[symmetric] FVars_term_def)
+  apply (rule impI)
+  apply (rule TT_total_abs_eq_iffs[THEN iffD2])
+  apply (rule alpha_bijs)
+       apply (rule assms)+
+   apply assumption+
+  apply (rule alpha_refls)
+  done
+
+lemmas permute_cong_ids = permute_congs[OF _ _ bij_id supp_id_bound, unfolded permute_ids, unfolded id_def]
+
+lemma existential_induct:
+  assumes IHs: "\<And>x \<rho>. \<rho> \<in> Param \<Longrightarrow> \<exists>y. term_ctor y = term_ctor x \<and>
+    ((\<forall>z. z \<in> set4_term_pre y \<longrightarrow> (\<forall>\<rho>\<in>Param. P z \<rho>)) \<and>
+     (\<forall>z. z \<in> set5_term_pre y \<longrightarrow> (\<forall>\<rho>\<in>Param. P z \<rho>)) \<and>
+     (\<forall>z. z \<in> set6_term_pre y \<longrightarrow> (\<forall>\<rho>\<in>Param. P z \<rho>)) \<longrightarrow> P (term_ctor y) \<rho>)"
+  shows "\<forall>\<rho>\<in>Param. P z \<rho>"
+  apply (unfold ball_conj_distrib)?
+  apply (rule subshape_induct[of "\<lambda>x. \<forall>\<rho>\<in>Param. P (TT_abs x) \<rho>" "TT_rep z", unfolded TT_abs_rep])
+  apply (rule ballI)
+  subgoal for x \<rho>
+    apply (rule raw_term.exhaust[of x])
+    apply hypsubst_thin
+    apply (rule iffD2[OF arg_cong2[OF _ refl, of _ _ P]])
+     apply (rule TT_total_abs_eq_iffs[THEN iffD2])
+     apply (rule alpha_term.intros)
+            apply (rule bij_id supp_id_bound id_on_id eq_on_refl)+
+     apply (unfold permute_raw_ids)
+     apply (rule iffD2[OF term_pre.mr_rel_map(3)])
+                apply (rule supp_id_bound bij_id)+
+     apply (unfold inv_id id_o o_id relcompp_conversep_Grp term_pre.mr_rel_id[symmetric])
+     apply (rule term_pre.rel_refl_strong)
+        apply (rule TT_rep_abs_syms[unfolded comp_apply[symmetric, of TT_rep TT_abs]])+
+    apply (unfold id_hid_o_hid)
+    apply (unfold hidden_id_def)
+    apply (subst term_pre.map_comp[symmetric])
+      apply (rule supp_id_bound bij_id)+
+    apply (unfold term_ctor_def[symmetric])
+    apply (drule IHs)
+    apply (erule exE)
+    apply (erule conjE)
+    apply (drule sym)
+    apply (rule iffD2[OF arg_cong2[OF _ refl, of _ _ P]])
+    apply assumption
+    apply (erule mp)
+     apply (drule TT_inject0s[THEN iffD1])
+    apply (erule exE conjE)+
+    apply hypsubst
+    apply (subst (asm) term_pre.set_map, (rule supp_id_bound bij_id)+)+
+    apply (subst term_pre.set_map, (rule supp_id_bound bij_id | assumption)+)+
+    apply (unfold image_comp[unfolded comp_def] image_id)
+    (* REPEAT_DETERM *)
+    apply (rule conjI)?
+     apply (rule allI)
+     apply (rule impI)
+     apply (erule imageE)
+     apply hypsubst
+     apply (subst permute_abs, (rule supp_id_bound bij_id | assumption)+)?
+     apply (drule set_subshapess set_subshape_permutess[rotated -1], assumption)
+      apply assumption+
+    (* repeated *)
+    apply (rule conjI)?
+     apply (rule allI)
+     apply (rule impI)
+     apply (erule imageE)
+     apply hypsubst
+          apply (subst permute_abs, (rule supp_id_bound bij_id | assumption)+)?
+     apply (drule set_subshape_permutess[rotated -1])
+    prefer 3 (* 2 * nvars + 1 *)
+      apply assumption+
+    (* repeated *)
+    apply (rule conjI)?
+     apply (rule allI)
+     apply (rule impI)
+     apply (erule imageE)
+     apply hypsubst
+    apply (subst permute_abs, (rule supp_id_bound bij_id | assumption)+)?
+    apply (unfold id_def)[1]
+    apply (drule set_subshapess, assumption)
+    (* END REPEAT_DETERM *)
+    done
+  done
+
+lemma fresh_induct_param:
+  fixes K::"'p \<Rightarrow> 'a::var_term_pre set"
+  assumes "\<And>\<rho>. \<rho> \<in> Param \<Longrightarrow> |K \<rho>| <o |UNIV::'a set|"
+  and IHs: "\<And>x \<rho>.
+    (\<And>z \<rho>. z \<in> set4_term_pre x \<Longrightarrow> \<rho> \<in> Param \<Longrightarrow> P z \<rho>) \<Longrightarrow>
+    (\<And>z \<rho>. z \<in> set5_term_pre x \<Longrightarrow> \<rho> \<in> Param \<Longrightarrow> P z \<rho>) \<Longrightarrow>
+    (\<And>z \<rho>. z \<in> set6_term_pre x \<Longrightarrow> \<rho> \<in> Param \<Longrightarrow> P z \<rho>) \<Longrightarrow>
+    set2_term_pre x \<inter> K \<rho> = {} \<Longrightarrow> set3_term_pre x \<inter> K \<rho> = {} \<Longrightarrow>
+    \<rho> \<in> Param \<Longrightarrow> P (term_ctor x) \<rho>"
+shows "\<forall>\<rho>\<in>Param. P z \<rho>"
+  apply (rule existential_induct[of _ P z])
+  subgoal for x \<rho>
+    apply (rule fresh_cases[of "K \<rho>" "term_ctor x"])
+     apply (erule assms)
+    apply (rule exI)
+    apply (rule conjI)
+     apply (erule sym)
+    apply (rule impI)
+    apply (erule conjE)+
+    apply (rule IHs)
+    (* for i in [~rec_vars - 2 .. ~3] *)
+        apply (rotate_tac -5)
+        apply (erule allE)
+        apply (erule impE)
+         apply assumption
+        apply (erule ballE)
+         apply assumption
+        apply (rotate_tac -1)
+        apply (erule contrapos_np)
+        apply assumption
+    (* repeated *)
+        apply (rotate_tac -4)
+        apply (erule allE)
+        apply (erule impE)
+         apply assumption
+        apply (erule ballE)
+         apply assumption
+        apply (rotate_tac -1)
+        apply (erule contrapos_np)
+        apply assumption
+    (* repeated *)
+        apply (rotate_tac -3)
+        apply (erule allE)
+        apply (erule impE)
+         apply assumption
+        apply (erule ballE)
+         apply assumption
+        apply (rotate_tac -1)
+        apply (erule contrapos_np)
+        apply assumption
+    (* END REPEAT_DETERM *)
+      apply assumption+
+    done
+  done
+
+lemma nnoclash_noclashs:
+  "noclash_term x = noclash_raw_term (map_term_pre id id id TT_rep TT_rep TT_rep x)"
+  apply (unfold noclash_term_def noclash_raw_term_def)
+  apply (subst term_pre.set_map, (rule supp_id_bound bij_id)+)+
+  apply (unfold image_id image_comp[unfolded comp_def] FVars_term_def[symmetric])
+  apply (rule refl)
+  done
+
+end
